a fragment for pending set to track number of pendings out there. State resource to track good/bad state.

theories/examples/susp_correctness/resource_algebras.v
@@ -1,7 +1,8 @@
 From auth.prelude Require Import stdpp.
 From auth.rel_logic_tern_susp Require Export model.
-From iris.algebra Require Import gmap auth excl.
+From iris.algebra Require Import gmap auth excl gset csum.
 From iris.algebra.lib Require Import dfrac_agree.
+
 
 (* Nat is going to be the id assigned by the verifier. We are going to show that
   for some value in the verifier's map, the ctr must be > 0. These values are either
@@ -10,60 +11,89 @@ From iris.algebra.lib Require Import dfrac_agree.
   have been seen (because of flush_buf_stream), and since this is the highest
   id, and children's ids are higher, we have a contradiction. *)
 Definition visited_state_mapUR :=
-  authUR (gmap gname (dfrac_agreeR (optionUR (prodUR natO (optionUR unitO))))).
+  authUR (gmap gname (csumR (exclR (optionO natO)) (agreeR natO))).
 Definition visited_done_mapUR :=
   authUR (gmap gname (agreeR natO)).
+Definition pending_setUR :=
+  authUR (gset_disjUR gname).
+Definition pendingnUR := dfrac_agreeR natO.
 Class visited_mapG Σ := VisitedMapG {
   visited_state_inG :> inG Σ visited_state_mapUR;
   visited_done_inG :> inG Σ visited_done_mapUR;
+  pending_set_inG :> inG Σ pending_setUR;
+  pendingn_inG :> inG Σ pendingnUR;
   visited_state_name : gname;
   visited_done_name : gname;
+  pending_set_name : gname;
+  pendingnG_name : gname;
 }.
 
 Section visited_map_res.
   Context `{!visited_mapG Σ}.
 
-  Definition state_val_type := dfrac_agreeR (option (nat * option unit)).
+  Definition state_val_type := csumR (exclR (optionO natO)) (agreeR natO).
   Definition state_mapg_type := gmap gname state_val_type.
   Definition done_mapg_type := gmap gname (agreeR natO).
+  Definition pending_setg_type := gset gname.
+
+  Definition pencount_frag (pn : nat) : iProp Σ :=
+    own pendingnG_name (to_dfrac_agree (DfracOwn (1/2)) pn).
 
   Definition pending_val : state_val_type :=
-    to_dfrac_agree (DfracOwn (1/2)%Qp) None.
-
-  Definition pending_val_full : state_val_type :=
-    to_dfrac_agree (DfracOwn 1) None.
+    Cinl (Excl None).
 
   Definition done_val n : state_val_type :=
-    to_dfrac_agree (DfracOwn 1) (Some (n, None)).
+    Cinl (Excl (Some n)).
 
   Definition finished_val n : state_val_type :=
-    to_dfrac_agree DfracDiscarded (Some (n, Some ())).
+    Cinr (to_agree n).
+
+  Definition penset_frag (γs : gset gname) : iProp Σ :=
+    own pending_set_name (◯ GSet γs).
 
   Definition visited_coherent (m : state_mapg_type) (d : done_mapg_type) : Prop :=
     ∀ γ, d !! γ ≠ None →
       ∃ n, m !! γ = Some (done_val n) ∨ m !! γ = Some (finished_val n).
 
-  Definition visited_mapg_auth (m : state_mapg_type) (d : done_mapg_type) : iProp Σ :=
+  Definition pending_coherent (m : state_mapg_type) (ps : pending_setg_type) (pending_n : nat) : Prop :=
+    pending_n = size ps ∧
+      ∀ γ, m !! γ = Some pending_val → γ ∈ ps.
+
+  Definition visited_mapg_auth (m : state_mapg_type) (d : done_mapg_type) (ps : pending_setg_type) (pending_n : nat) : iProp Σ :=
     own visited_state_name (● m) ∗ own visited_done_name (● d) ∗
-    ⌜visited_coherent m d⌝.
+    own pending_set_name (● GSet ps) ∗ pencount_frag pending_n ∗
+    ⌜visited_coherent m d⌝ ∗ ⌜pending_coherent m ps pending_n⌝.
 
   Definition visited_map_update_pending
-      (m : state_mapg_type) (d : done_mapg_type) γ : iProp Σ :=
-    own visited_state_name (● <[ γ := pending_val_full ]>m) ∗
+      (m : state_mapg_type) (d : done_mapg_type) (ps : pending_setg_type) pn (γs : gset gname) : iProp Σ :=
+    let m' := set_fold (λ γ m, <[ γ := pending_val ]>m) m γs in
+    let ps' := ps ∪ γs in
+    own visited_state_name (● m') ∗
     own visited_done_name (● d) ∗
-    ⌜visited_coherent (<[ γ := pending_val_full ]>m) d⌝.
+    own pending_set_name (● GSet ps') ∗ pencount_frag (pn + size γs) ∗
+    ⌜visited_coherent m' d⌝ ∗
+    ⌜pending_coherent m' ps' (pn + size γs)⌝.
 
   Definition visited_map_update_done
-      (m : state_mapg_type) (d : done_mapg_type) γ n : iProp Σ :=
+      (m : state_mapg_type) (d : done_mapg_type) (ps : pending_setg_type) pn γ n : iProp Σ :=
     own visited_state_name (● <[ γ := done_val n ]>m) ∗
     own visited_done_name (● <[ γ := to_agree n ]>d) ∗
-    ⌜visited_coherent (<[ γ := done_val n ]>m) (<[ γ := to_agree n ]>d)⌝.
+    own pending_set_name (● GSet ps) ∗ pencount_frag pn ∗
+    ⌜visited_coherent (<[ γ := done_val n ]>m) (<[ γ := to_agree n ]>d)⌝ ∗
+    ⌜pending_coherent (<[ γ := done_val n ]>m) ps pn⌝.
 
   Definition visited_map_update_finished
-      (m : state_mapg_type) (d : done_mapg_type) γ n : iProp Σ :=
+      (m : state_mapg_type) (d : done_mapg_type) (ps : pending_setg_type) pn γ n : iProp Σ :=
     own visited_state_name (● <[ γ := finished_val n ]>m) ∗
     own visited_done_name (● d) ∗
-    ⌜visited_coherent (<[ γ := finished_val n ]>m) d⌝.
+    own pending_set_name (● GSet ps) ∗ pencount_frag pn ∗
+    ⌜visited_coherent (<[ γ := finished_val n ]>m) d⌝ ∗
+    ⌜pending_coherent (<[ γ := finished_val n ]>m) ps pn⌝.
+
+  Definition visited_mapg_pending_removed (m : state_mapg_type) (d : done_mapg_type) (ps : pending_setg_type) (pending_n : nat) (γs : gset gname) : iProp Σ :=
+    own visited_state_name (● m) ∗ own visited_done_name (● d) ∗
+    own pending_set_name (● GSet (ps ∖ γs)) ∗ pencount_frag (pending_n - size γs) ∗
+    ⌜visited_coherent m d⌝ ∗ ⌜pending_coherent m (ps ∖ γs) (pending_n - size γs)⌝.
 
   Definition visit_pending γ : iProp Σ :=
     own visited_state_name (◯ {[ γ := pending_val ]}).
@@ -85,62 +115,92 @@ Section visited_map_res.
     Persistent (visit_finished γ n).
   Proof. rewrite /visit_finished /finished_val. apply _. Qed.
 
-  Local Lemma pending_val_split :
-    pending_val ⋅ pending_val ≡ pending_val_full.
+  Lemma pn_agree pn pn' :
+    pencount_frag pn -∗ pencount_frag pn' -∗ ⌜pn = pn'⌝ ∗ pencount_frag pn ∗ pencount_frag pn'.
   Proof.
-    rewrite /pending_val /pending_val_full -dfrac_agree_op dfrac_op_own Qp.half_half //.
+    iIntros "H1 H2". rewrite /pencount_frag. iCombine "H1 H2" as "H".
+    iDestruct (own_valid with "H") as %Hv%dfrac_agree_op_valid_L.
+    destruct Hv as [_ ->].
+    iDestruct "H" as "[H1 H2]". by iFrame.
   Qed.
 
-  Lemma visited_insert m d γ :
-    m !! γ = None →
-    visited_mapg_auth m d ==∗
-      visited_map_update_pending m d γ ∗ visit_pending γ ∗ visit_pending γ.
+  Lemma pn_update pn pn' :
+    pencount_frag pn -∗ pencount_frag pn ==∗ pencount_frag pn' ∗ pencount_frag pn'.
   Proof.
-    iIntros (Hfresh) "(Hms & Hd & %Hcoh)".
-    rewrite /visited_map_update_pending /visit_pending.
+    iIntros "H1 H2". rewrite /pencount_frag. iCombine "H1 H2" as "H".
+    iMod (own_update with "H") as "[H1 H2]"; last by iFrame.
+    apply frac_agree_update_2. by rewrite Qp.half_half.
+  Qed.
+
+  Lemma visited_insert m d ps pn :
+    visited_mapg_auth m d ps pn ∗ pencount_frag pn ==∗
+      ∃ γ,
+        visited_map_update_pending m d ps pn {[γ]} ∗ pencount_frag (pn+1) ∗
+          visit_pending γ ∗ penset_frag {[γ]}.
+  Proof.
+    iIntros "((Hms & Hd & Hps & Hpn1 & %Hcoh & %Hpcoh) & Hpn2)".
+    set (γ := fresh (dom m ∪ ps)).
+    assert (γ ∉ (dom m ∪ ps : gset gname)) as Hfr by apply is_fresh.
+    rewrite not_elem_of_union in Hfr.
+    destruct Hfr as [Hfm%not_elem_of_dom Hfps].
     iMod (own_update _ _
-      (● <[γ := pending_val_full]>m
-        ⋅ (◯ {[γ := pending_val]} ⋅ ◯ {[γ := pending_val]}))
-      with "Hms") as "[$ [$ $]]".
-    { rewrite -auth_frag_op singleton_op pending_val_split.
-      apply auth_update_alloc, alloc_singleton_local_update; [done|].
-      rewrite /pending_val_full pair_valid; done. }
-    iFrame "Hd". iPureIntro.
-    intros γ' Hdγ'. destruct (decide (γ' = γ)) as [-> | Hne].
-    - destruct (Hcoh γ Hdγ') as (n & [Heq | Heq]); rewrite Hfresh in Heq; discriminate.
-    - rewrite lookup_insert_ne; [|done]. by apply Hcoh.
+      (● <[γ := pending_val]>m ⋅ ◯ {[γ := pending_val]})
+      with "Hms") as "[Hms' Hp]".
+    { apply auth_update_alloc, alloc_singleton_local_update; done. }
+    iMod (own_update _ _ (● GSet ({[γ]} ∪ ps) ⋅ ◯ GSet {[γ]}) with "Hps") as "[Hps' Hpsf]".
+    { apply auth_update_alloc, gset_disj_alloc_empty_local_update. set_solver. }
+    iMod (pn_update pn (pn+1) with "Hpn1 Hpn2") as "[Hpn1 Hpn2]".
+    iModIntro. iExists γ.
+    rewrite /visited_map_update_pending /visit_pending /penset_frag.
+    rewrite set_fold_singleton size_singleton (union_comm_L ps {[γ]}) /=.
+    iFrame "Hms' Hd Hps' Hpn1 Hpn2 Hp Hpsf".
+    iPureIntro. split.
+    - intros γ' Hdγ'. destruct (decide (γ' = γ)) as [-> | Hne].
+      + destruct (Hcoh γ Hdγ') as (n & [Heq | Heq]); rewrite Hfm in Heq; discriminate.
+      + rewrite lookup_insert_ne; [|done]. by apply Hcoh.
+    - destruct Hpcoh as [Hsize Hl]. split.
+      + rewrite size_union; last set_solver. rewrite size_singleton. lia.
+      + intros γ' Hγ'. destruct (decide (γ' = γ)) as [-> | Hne].
+        * set_solver.
+        * rewrite lookup_insert_ne in Hγ'; [|done].
+          apply elem_of_union; right. by apply Hl.
   Qed.
 
-  Lemma visited_transition_done m d γ n :
+  Lemma visited_transition_done m d ps pn γ n :
     d !! γ = None →
-    visited_mapg_auth m d -∗ visit_pending γ -∗ visit_pending γ
-    ==∗ visited_map_update_done m d γ n ∗ visit_done γ n.
+    visited_mapg_auth m d ps pn -∗ visit_pending γ
+    ==∗ visited_map_update_done m d ps pn γ n ∗ visit_done γ n.
   Proof.
-    iIntros (Hdγ) "(Hms & Hd & %Hcoh) H1 H2".
+    iIntros (Hdγ) "(Hms & Hd & Hps & Hpn & %Hcoh & %Hpcoh) H1".
     rewrite /visited_map_update_done /visit_done /visit_reached_done.
-    iMod (own_update_3 _ _ _ _
+    iMod (own_update_2 _ _ _
       (● <[γ := done_val n]>m ⋅ ◯ {[γ := done_val n]})
-      with "Hms H1 H2") as "[$ Hf]".
-    { rewrite -assoc -auth_frag_op singleton_op pending_val_split.
-      apply auth_update, singleton_local_update_any.
-      intros x Hx. apply exclusive_local_update.
-      rewrite /done_val pair_valid; done. }
+      with "Hms H1") as "[$ Hf]".
+    { apply auth_update, singleton_local_update_any.
+      intros x Hx. unfold pending_val.
+      apply (exclusive_local_update _ (done_val n)). done. }
     iMod (own_update _ _
       (● <[γ := to_agree n]>d ⋅ ◯ {[γ := to_agree n]})
       with "Hd") as "[$ #$]".
     { apply auth_update_alloc, alloc_singleton_local_update; done. }
-    iFrame "Hf". iPureIntro.
-    intros γ' Hdγ'. destruct (decide (γ' = γ)) as [-> | Hne].
-    - exists n. left. by rewrite lookup_insert.
-    - rewrite lookup_insert_ne; [|done]. apply Hcoh.
-      rewrite lookup_insert_ne in Hdγ'; done.
+    iFrame "Hps Hpn Hf". iPureIntro. split.
+    - intros γ' Hdγ'. destruct (decide (γ' = γ)) as [-> | Hne].
+      + exists n. left. by rewrite lookup_insert.
+      + rewrite lookup_insert_ne; [|done]. apply Hcoh.
+        rewrite lookup_insert_ne in Hdγ'; done.
+    - destruct Hpcoh as [Hsize Hl]. split; [exact Hsize|].
+      intros γ' Hγ'. destruct (decide (γ' = γ)) as [-> | Hne].
+      + exfalso. rewrite lookup_insert in Hγ'.
+        rewrite /done_val /pending_val in Hγ'.
+        by inversion Hγ'.
+      + rewrite lookup_insert_ne in Hγ'; [|done]. by apply Hl.
   Qed.
 
-  Lemma visited_transition_finished m d γ n :
-    visited_mapg_auth m d -∗ visit_done γ n
-    ==∗ visited_map_update_finished m d γ n ∗ visit_finished γ n.
+  Lemma visited_transition_finished m d ps pn γ n :
+    visited_mapg_auth m d ps pn -∗ visit_done γ n
+    ==∗ visited_map_update_finished m d ps pn γ n ∗ visit_finished γ n.
   Proof.
-    iIntros "(Hms & Hd & %Hcoh) [Hsfrag #Hreached]".
+    iIntros "(Hms & Hd & Hps & Hpn & %Hcoh & %Hpcoh) [Hsfrag #Hreached]".
     rewrite /visited_map_update_finished /visit_finished /visit_reached_done.
     iDestruct (own_valid_2 with "Hd Hreached") as %Hv.
     apply auth_both_valid_discrete in Hv as [Hincl _].
@@ -151,12 +211,18 @@ Section visited_map_res.
       (● <[γ := finished_val n]>m ⋅ ◯ {[γ := finished_val n]})
       with "Hms Hsfrag") as "[$ $]".
     { apply auth_update, singleton_local_update_any.
-      intros x Hx. apply exclusive_local_update.
-      rewrite /finished_val pair_valid; done. }
-    iFrame "Hd Hreached". iPureIntro.
-    intros γ' Hdγ'. destruct (decide (γ' = γ)) as [-> | Hne].
-    - exists n. right. by rewrite lookup_insert.
-    - rewrite lookup_insert_ne; [|done]. by apply Hcoh.
+      intros x Hx. unfold done_val.
+      apply (exclusive_local_update _ (finished_val n)). done. }
+    iFrame "Hd Hps Hpn Hreached". iPureIntro. split.
+    - intros γ' Hdγ'. destruct (decide (γ' = γ)) as [-> | Hne].
+      + exists n. right. by rewrite lookup_insert.
+      + rewrite lookup_insert_ne; [|done]. by apply Hcoh.
+    - destruct Hpcoh as [Hsize Hl]. split; [exact Hsize|].
+      intros γ' Hγ'. destruct (decide (γ' = γ)) as [-> | Hne].
+      + exfalso. rewrite lookup_insert in Hγ'.
+        rewrite /finished_val /pending_val in Hγ'.
+        by inversion Hγ'.
+      + rewrite lookup_insert_ne in Hγ'; [|done]. by apply Hl.
   Qed.
 
   Lemma visit_done_keep γ n :
@@ -178,8 +244,8 @@ Section visited_map_res.
     iIntros "[H1 [H2 _]]". iCombine "H1 H2" as "H".
     iDestruct (own_valid with "H") as %Hv. iPureIntro.
     rewrite auth_frag_valid singleton_valid in Hv.
-    rewrite /pending_val /done_val in Hv.
-    by apply dfrac_agree_op_valid_L in Hv as [_ ?].
+    rewrite /pending_val /done_val -Cinl_op in Hv.
+    apply (@Cinl_valid _ (agreeR natO)), exclusive_l in Hv; done.
   Qed.
 
   Lemma visited_invalid_2 γ n :
@@ -189,8 +255,7 @@ Section visited_map_res.
     iIntros "[H1 [H2 _]]". iCombine "H1 H2" as "H".
     iDestruct (own_valid with "H") as %Hv. iPureIntro.
     rewrite auth_frag_valid singleton_valid in Hv.
-    rewrite /pending_val /finished_val in Hv.
-    by apply dfrac_agree_op_valid_L in Hv as [_ ?].
+    rewrite /pending_val /finished_val in Hv. done.
   Qed.
 
   Lemma visited_invalid_3 γ n1 n2 :
@@ -200,8 +265,7 @@ Section visited_map_res.
     iIntros "[[H1 _] [H2 _]]". iCombine "H1 H2" as "H".
     iDestruct (own_valid with "H") as %Hv. iPureIntro.
     rewrite auth_frag_valid singleton_valid in Hv.
-    rewrite /done_val /finished_val in Hv.
-    apply dfrac_agree_op_valid_L in Hv as [_ Heq]. by simplify_eq.
+    rewrite /done_val /finished_val in Hv. done.
   Qed.
 
   Lemma visited_reached_done_agree γ n1 n2 :
@@ -214,11 +278,11 @@ Section visited_map_res.
     by apply to_agree_op_inv_L in Hv.
   Qed.
 
-  Lemma get_visit_reached_done γ n m d :
+  Lemma get_visit_reached_done γ n m d ps pn :
     d !! γ = Some (to_agree n) →
-    visited_mapg_auth m d ==∗ visited_mapg_auth m d ∗ visit_reached_done γ n.
+    visited_mapg_auth m d ps pn ==∗ visited_mapg_auth m d ps pn ∗ visit_reached_done γ n.
   Proof.
-    iIntros (Hd) "(Hms & Hd & %Hcoh)".
+    iIntros (Hd) "(Hms & Hd & Hps & Hpn & %Hcoh & %Hpcoh)".
     rewrite /visit_reached_done.
     iMod (own_update _ _ (● d ⋅ ◯ {[γ := to_agree n]}) with "Hd") as "[Hd #Hr]".
     { apply auth_update_dfrac_alloc; [apply _|].
@@ -227,10 +291,10 @@ Section visited_map_res.
     iModIntro. by iFrame "∗ # %".
   Qed.
 
-  Lemma visited_reached_done_invalid γ n m d :
-    visited_mapg_auth m d -∗ visit_reached_done γ n -∗ visit_pending γ -∗ False.
+  Lemma visited_reached_done_invalid γ n m d ps pn :
+    visited_mapg_auth m d ps pn -∗ visit_reached_done γ n -∗ visit_pending γ -∗ False.
   Proof.
-    iIntros "(Hms & Hd & %Hcoh) Hreached Hpending".
+    iIntros "(Hms & Hd & Hps & Hpn & %Hcoh & %Hpcoh) Hreached Hpending".
     rewrite /visit_reached_done /visit_pending.
     iDestruct (own_valid_2 with "Hd Hreached") as %Hvd.
     apply auth_both_valid_discrete in Hvd as [Hincl_d _].
@@ -244,10 +308,20 @@ Section visited_map_res.
     iPureIntro. destruct Hmγ as [Hmγ | Hmγ]; rewrite Hmγ in Hym;
       apply Some_equiv_inj in Hym; rewrite -Hym in Hle;
       apply Some_included in Hle as [Heq | Hle].
-    - destruct Heq as [_ Hv]. apply (inj to_agree) in Hv. by inversion Hv.
-    - apply dfrac_agree_included in Hle as [_ Heqv]. by inversion Heqv.
-    - destruct Heq as [_ Hv]. apply (inj to_agree) in Hv. by inversion Hv.
-    - apply dfrac_agree_included in Hle as [_ Heqv]. by inversion Heqv.
+    - rewrite /pending_val /done_val in Heq.
+      apply (inj Cinl), (inj Excl) in Heq. by inversion Heq.
+    - rewrite /pending_val /done_val in Hle.
+      apply csum_included in Hle as [Hbot | [(?&?& Heq1 & Heq2 & Hinc) | (?&?& Heq1 & _ & _)]].
+      + by inversion Hbot.
+      + injection Heq1 as <-. injection Heq2 as <-.
+        exfalso. apply (exclusive_included (Excl None) (Excl (Some n'))); done.
+      + by inversion Heq1.
+    - rewrite /pending_val /finished_val in Heq. by inversion Heq.
+    - rewrite /pending_val /finished_val in Hle.
+      apply csum_included in Hle as [Hbot | [(?&?& _ & Heq1 & _) | (?&?& Heq1 & _ & _)]].
+      + by inversion Hbot.
+      + by inversion Heq1.
+      + by inversion Heq1.
   Qed.
 
   Lemma visited_agree_n γ n1 n2 :
@@ -266,21 +340,80 @@ Section visited_map_res.
     iFrame.
   Qed.
 
+  Lemma pending_set_combine γs1 γs2 :
+    penset_frag γs1 ∗ penset_frag γs2 ⊣⊢ ⌜γs1 ## γs2⌝ ∗ penset_frag (γs1 ∪ γs2).
+  Proof.
+    rewrite /penset_frag. iSplit.
+    - iIntros "[H1 H2]". iCombine "H1 H2" as "H".
+      iDestruct (own_valid with "H") as %Hv%auth_frag_valid_1.
+      apply gset_disj_valid_op in Hv.
+      iSplit; [done|]. by rewrite gset_disj_union //.
+    - iIntros "[%Hdisj H]". rewrite -gset_disj_union // -own_op -auth_frag_op //.
+  Qed.
+
+  Lemma pending_set_remove m d ps pn γs :
+    visited_mapg_auth m d ps pn -∗ pencount_frag pn -∗ penset_frag γs -∗
+    ([∗ set] γ ∈ γs, ∃ n, visit_reached_done γ n) ==∗
+    visited_mapg_pending_removed m d ps pn γs ∗ pencount_frag (pn - size γs).
+  Proof.
+    iIntros "(Hms & Hd & Hps & Hpn1 & %Hcoh & %Hpcoh) Hpn2 Hfrag #Hreached".
+    iAssert (⌜∀ γ, γ ∈ γs → d !! γ ≠ None⌝)%I as %Hdγs.
+    { iIntros (γ Hin).
+      iDestruct (big_sepS_elem_of with "Hreached") as (n) "Hr"; first done.
+      iDestruct (own_valid_2 with "Hd Hr") as %Hv.
+      apply auth_both_valid_discrete in Hv as [Hincl _].
+      apply singleton_included_l in Hincl as (xd & Hxd & _).
+      iPureIntro. intros Heq. rewrite Heq in Hxd. inversion Hxd. }
+    rewrite /visited_mapg_pending_removed /penset_frag.
+    iCombine "Hps Hfrag" as "Hpsfull".
+    iDestruct (own_valid with "Hpsfull") as %Hv.
+    apply auth_both_valid_discrete in Hv as [Hincl%gset_disj_included _].
+    iMod (own_update with "Hpsfull") as "Hps'".
+    { apply auth_update_dealloc, gset_disj_dealloc_local_update. }
+    iMod (pn_update pn (pn - size γs) with "Hpn1 Hpn2") as "[Hpn1 Hpn2]".
+    iModIntro. iFrame "Hms Hd Hps' Hpn1 Hpn2". iPureIntro. split; first done.
+    destruct Hpcoh as [Hsz Hpcoh].
+    split.
+    - rewrite (size_difference _ _ Hincl) -Hsz //.
+    - intros γ' Hm. specialize (Hpcoh γ' Hm).
+      destruct (decide (γ' ∈ γs)) as [Hin | Hnin].
+      + exfalso. specialize (Hdγs _ Hin).
+        destruct (Hcoh γ' Hdγs) as (n & [Hmγ | Hmγ]); rewrite Hmγ in Hm;
+          rewrite /done_val /finished_val /pending_val in Hm;
+          by inversion Hm.
+      + by apply elem_of_difference.
+  Qed.
+
 End visited_map_res.
 
-Definition lg_mapUR := authR (gmapUR loc (agreeR (leibnizO gname))).
+(* Each [loc] in the lg_map is in one of two states:
+   - [Cinl (to_agree ())]   — explicitly unallocated (filled tauth leaf)
+   - [Cinr (to_agree γ)]    — allocated to [γ] (suspended tauth leaf)
+   Both states use [agreeR], so fragments are persistent and a single [loc]
+   cannot be in both states simultaneously ([Cinl · Cinr] is invalid). *)
+Definition lg_mapEntry := csumR (agreeR unitO) (agreeR (leibnizO gname)).
+Definition lg_mapUR := authR (gmapUR loc lg_mapEntry).
 Class lg_mapG Σ := Lg_mapG { lg_map_inG :> inG Σ lg_mapUR; lg_mapG_name : gname }.
 
 Section lg_map.
   Context `{!lg_mapG Σ}.
 
-  Definition lg_mapg_type := gmap loc (agree gname).
+  Definition lg_mapg_type := gmap loc lg_mapEntry.
 
   Definition lg_mapg_auth (m : lg_mapg_type) : iProp Σ :=
     own lg_mapG_name (● m).
 
   Definition lg_mapg_frag l γ : iProp Σ :=
-    own lg_mapG_name (◯ {[ l := to_agree γ ]}).
+    own lg_mapG_name (◯ {[ l := Cinr (to_agree γ) ]}).
+
+  Definition lg_mapg_unalloc l : iProp Σ :=
+    own lg_mapG_name (◯ {[ l := Cinl (to_agree ()) ]}).
+
+  Global Instance lg_mapg_frag_persistent l γ : Persistent (lg_mapg_frag l γ).
+  Proof. apply _. Qed.
+
+  Global Instance lg_mapg_unalloc_persistent l : Persistent (lg_mapg_unalloc l).
+  Proof. apply _. Qed.
 
   Lemma lg_mapg_agree l γ1 γ2 :
     lg_mapg_frag l γ1 -∗ lg_mapg_frag l γ2 -∗ ⌜γ1 = γ2⌝ ∗ lg_mapg_frag l γ1 ∗ lg_mapg_frag l γ2.
@@ -288,15 +421,38 @@ Section lg_map.
     rewrite /lg_mapg_frag. iIntros "H1 H2".
     iDestruct (own_valid_2 with "H1 H2") as %Hv.
     iFrame. iPureIntro.
-    rewrite -auth_frag_op auth_frag_valid singleton_op singleton_valid in Hv.
+    rewrite -auth_frag_op auth_frag_valid singleton_op singleton_valid -Cinr_op
+      Cinr_valid in Hv.
     fold_leibniz. by apply to_agree_op_inv_L in Hv.
+  Qed.
+
+  (* The two states are mutually exclusive at the same location. *)
+  Lemma lg_mapg_frag_unalloc_excl l γ :
+    lg_mapg_frag l γ -∗ lg_mapg_unalloc l -∗ False.
+  Proof.
+    rewrite /lg_mapg_frag /lg_mapg_unalloc. iIntros "H1 H2".
+    iDestruct (own_valid_2 with "H1 H2") as %Hv.
+    rewrite -auth_frag_op singleton_op auth_frag_valid singleton_valid in Hv.
+    done.
   Qed.
 
   Lemma lg_mapg_insert m l γ :
     m !! l = None →
-    lg_mapg_auth m ==∗ lg_mapg_auth (<[ l:= to_agree γ ]> m) ∗ lg_mapg_frag l γ.
+    lg_mapg_auth m ==∗
+      lg_mapg_auth (<[ l := Cinr (to_agree γ) ]> m) ∗ lg_mapg_frag l γ.
   Proof.
     rewrite /lg_mapg_auth /lg_mapg_frag. iIntros (Hfresh) "H".
+    iMod (own_update with "H") as "[$ $]"; last done.
+    apply auth_update_alloc.
+    by apply alloc_singleton_local_update.
+  Qed.
+
+  Lemma lg_mapg_insert_unalloc m l :
+    m !! l = None →
+    lg_mapg_auth m ==∗
+      lg_mapg_auth (<[ l := Cinl (to_agree ()) ]> m) ∗ lg_mapg_unalloc l.
+  Proof.
+    rewrite /lg_mapg_auth /lg_mapg_unalloc. iIntros (Hfresh) "H".
     iMod (own_update with "H") as "[$ $]"; last done.
     apply auth_update_alloc.
     by apply alloc_singleton_local_update.
@@ -476,3 +632,42 @@ Section intransit_res.
   Qed.
 
 End intransit_res.
+
+(* Tracks whether we are in the bad case or not. *)
+Definition stateUR := authUR (optionUR unitO).
+Class stateG Σ := StateG { state_inG :> inG Σ stateUR; stateG_name : gname }.
+
+Section state_res.
+  Context `{!stateG Σ}.
+
+  Definition state_car := optionUR unitO.
+
+  Definition state (o : state_car) := own stateG_name (●{DfracOwn (1/2)} o).
+  (* good_state represents the good case.
+    false_state represents the bad case.
+    Explained in more detail later. *)
+  Definition good_state := state None.
+  Definition false_state := state (Some ()).
+
+  Lemma state_agree (o o' : state_car) :
+    state o -∗ state o' -∗ ⌜o' = o⌝ ∗ state o ∗ state o'.
+  Proof.
+    rewrite /state. iIntros "H1 H2". iCombine "H1 H2" as "H".
+    iDestruct (own_valid with "H") as %Hv.
+    apply auth_auth_dfrac_op_valid in Hv as [_ [Heq _]].
+    iDestruct "H" as "[H1 H2]". iFrame.
+    iPureIntro. symmetry. apply leibniz_equiv. exact Heq.
+  Qed.
+
+  Lemma state_update_bad :
+    good_state -∗ good_state ==∗ false_state ∗ false_state.
+  Proof.
+    rewrite /good_state /false_state /state.
+    iIntros "H1 H2". iCombine "H1 H2" as "H".
+    iMod (own_update with "H") as "H".
+    { apply (auth_update_auth None (Some ()) (Some ())).
+      apply alloc_option_local_update. done. }
+    iDestruct "H" as "[H1 H2]". by iFrame.
+  Qed.
+
+End state_res.
